terms to eqTypes

src/Term.v
@@ -1,94 +1,136 @@
-From Coq Require Import Init.Nat.
-From Coq Require Import Strings.String.
-From Coq Require Import Arith.EqNat.
+From mathcomp Require Import all_ssreflect.
+Set Implicit Arguments.
+Unset Strict Implicit.
+Unset Printing Implicit Defensive.
 
-Definition eqb_string (x y : string) : bool :=
-  if string_dec x y then true else false.
+Section Term.
 
- (* literals should be of Datatype type, is not important for the moment*)
+  (* literals should be of Datatype type, is not important for the moment*)
+  Variable I B L: eqType.
+
+  (* Definition eqb_i (i1 i2 : I) : bool := *)
+  (*   bool_of_sumbool (Ieq_dec i1 i2). *)
+
 Inductive term : Type :=
-  | Iri (id: string)
-  | Lit (l : nat)
-  | Bnode (name : string).
+  | Iri (id: I) 
+  | Lit (l : L) 
+  | Bnode (name : B).
 
-Definition is_lit (n : term) : bool :=
-  (match n with
+
+Definition is_lit (t : term ) :=
+  (match t with
    | Lit _ => true
    | _ => false
    end).
 
-Definition is_iri (n : term) : bool :=
-  (match n with
+Definition is_iri (t : term ) : bool :=
+  (match t with
    | Iri _ => true
    | _ => false
    end).
 
-Definition is_bnode (n : term) : bool :=
-  (match n with
+Definition is_bnode (t : term ) : bool :=
+  (match t with
    | Bnode _ => true
    | _ => false
    end).
 
-Definition eqb_term (n1 n2 : term) : bool :=
-  (match n1, n2 with
-   | (Iri id), (Iri id2) => eqb id id2
-   | (Lit l),(Lit l2) => l =? l2
-   | (Bnode b),(Bnode b2) => eqb b b2
+
+Definition eqb_term (t1 t2 : term) : bool :=
+  (match t1, t2 with
+   | (Iri id1), (Iri id2) => id1 == id2
+   | (Lit l1),(Lit l2) => l1 == l2
+   | (Bnode b1),(Bnode b2) => b1 == b2
    | _,_ => false
    end).
 
-Theorem eq_nat_eq_lit : forall (n1 n2:nat) , (n1 = n2) <-> (Lit n1) = (Lit n2).
+(* Theorem eq_nat_in_set : forall (n1 n2:nat) (p: n1 = n2), (set_In n1 L) -> set_In n2 L. *)
+(* Proof. intros. symmetry in p. rewrite p. apply H. *)
+(* Qed. *)
+
+(* Theorem eq_nat_eq_in_set : forall (n1 n2:nat) (H: n1 = n2), set_In n1 L = set_In n2 L. *)
+(* Proof. intros. rewrite H. reflexivity. Qed. *)
+
+(* Theorem eq_p_eq_in_set : forall (n : nat) (p1 : set_In n L) (p2 : set_In n L), p1 = p2. *)
+(*   Proof. intros. revert n p1 p2. induction L ; cbn. intros _ []. *)
+
+(* Theorem eq_nat_eq_lit : forall (n1 n2:nat), *)
+(*     (n1 = n2) <-> (@Lit n1 (set_mem Nat.eq_dec) n1 L) = (@Lit n2 (set_mem Nat.eq_dec n2 L)). *)
+(* Proof. split; intros H. *)
+(*   - rewrite H. reflexivity. *)
+(*   - injection H as H2. apply H2. *)
+(* Qed. *)
+
+Theorem eq_l_eq_lit : forall (l1 l2:L),
+    (l1 = l2) <-> (Lit l1)  = (Lit l2).
 Proof. split; intros H.
   - rewrite H. reflexivity.
   - injection H as H2. apply H2.
 Qed.
 
-Theorem eq_string_eq_iri : forall (s1 s2:string) , (s1 = s2) <-> (Iri s1) = (Iri s2).
+Theorem eq_i_eq_iri : forall (i1 i2:I) ,
+    (i1 = i2) <-> (Iri i1) = (Iri i2).
 Proof. split; intros H.
   - rewrite H. reflexivity.
   - injection H as H2. apply H2.
 Qed.
 
-Theorem eq_string_eq_bnode : forall (s1 s2:string) , (s1 = s2) <-> (Bnode s1) = (Bnode s2).
+Theorem eq_b_eq_bnode : forall (b1 b2:B) ,
+    (b1 = b2) <-> (Bnode b1) = (Bnode b2).
 Proof. split; intros H.
   - rewrite H. reflexivity.
   - injection H as H2. apply H2.
 Qed.
 
-Theorem eq_dec_term : forall (t1 t2: term),
-  {t1 = t2} + {t1 <> t2}.
-Proof. decide equality.
-  + apply string_dec.
-  + decide equality.
-  + apply string_dec.
+(* Theorem eq_dec_term : forall (t1 t2: term), *)
+(*   {t1 = t2} + {t1 <> t2}. *)
+(* Proof. decide equality. *)
+(*        - apply eqVneq. *)
+
+(*   (try decide equality); (try apply string_dec); (try decide equality). Qed. *)
+
+(* Theorem eqb_term_refl : forall (t1 : term), *)
+(*   eqb_term t1 t1 = true. *)
+(* Proof. destruct t1 as []; simpl. *)
+(*   - apply eqb_refl. *)
+(*   - symmetry. apply beq_nat_refl. *)
+(*   - apply eqb_refl. *)
+(* Qed. *)
+
+(* Definition term_eqType : eqType := @Equality.Pack term eqb_term. *)
+
+Lemma term_eqP : Equality.axiom eqb_term.
+Proof.
+  rewrite /Equality.axiom => x y.
+  apply: (iffP idP) => //= [| ->]; rewrite /eqb_term; last by case y.
+  case: x y=> [i1|l1|b1] [i2|l2|b2]=> //.
+  rewrite -eq_i_eq_iri. by apply /eqP.
+  rewrite -eq_l_eq_lit. by apply /eqP.
+  rewrite -eq_b_eq_bnode. by apply /eqP.
 Qed.
 
-Theorem eqb_term_refl : forall (t1 : term),
-  eqb_term t1 t1 = true.
-Proof. destruct t1 as []; simpl.
-  - apply eqb_refl.
-  - symmetry. apply beq_nat_refl.
-  - apply eqb_refl.
-Qed.
+Canonical term_eqType := EqType term (EqMixin term_eqP).
 
-Theorem eqb_eq_term : forall (t1 t2 : term),
-  eqb_term t1 t2 = true <-> t1 = t2.
-Proof. split; intros H.
-  - destruct t1,t2 as [] ; 
-    try reflexivity ;
-    try discriminate; simpl in H.
-    + apply eqb_eq in H. rewrite H. apply eq_string_eq_iri. reflexivity.
-    + apply beq_nat_true in H. rewrite H. apply eq_nat_eq_lit. reflexivity.
-    + apply eqb_eq in H. apply eq_string_eq_bnode. apply H.
-  - rewrite H. apply eqb_term_refl.
-Qed.
-   
-Theorem eqb_neq_term : forall (t1 t2 : term),
-  eqb_term t1 t2 = false <-> t1 <> t2.
-Proof. split.
-  - intros H contra. rewrite contra in H. rewrite eqb_term_refl in H. discriminate H.
-  - intros H. unfold not in H. rewrite <- eqb_eq_term in H. destruct (eqb_term t1 t2) as [].
-    + exfalso. apply H. reflexivity.
-    + reflexivity.
-Qed.
+(* Theorem eqb_eq_term : forall (t1 t2 : term), *)
+(*   eqb_term t1 t2 <-> t1 = t2. *)
+(* Proof. split; intros H. *)
+(*   - destruct t1,t2 as [] ;  *)
+(*     try reflexivity ; *)
+(*     try discriminate; simpl in H. *)
+(*     + apply eq_i_eq_iri. apply H. apply eqb_eq in H. rewrite H. reflexivity. apply eq_string_eq_iri. reflexivity. *)
+(*     + apply beq_nat_true in H. rewrite H. apply eq_nat_eq_lit. reflexivity. *)
+(*     + apply eqb_eq in H. apply eq_string_eq_bnode. apply H. *)
+(*   - rewrite H. apply eqb_term_refl. *)
+(* Qed. *)
 
+
+(* Theorem eqb_neq_term : forall (t1 t2 : term), *)
+(*   eqb_term t1 t2 = false <-> t1 <> t2. *)
+(* Proof. split. *)
+(*   - intros H contra. rewrite contra in H. rewrite eqb_term_refl in H. discriminate H. *)
+(*   - intros H. unfold not in H. rewrite <- eqb_eq_term in H. destruct (eqb_term t1 t2) as []. *)
+(*     + exfalso. apply H. reflexivity. *)
+(*     + reflexivity. *)
+(* Qed. *)
+
+End Term.
